code/rsapss/Hacl.Spec.Bignum.Montgomery.fsti
@@ -14,11 +14,6 @@ module M = Hacl.Spec.Montgomery.Lemmas
 ///
 ///  Precomputed constants for Montgomery arithmetic
 ///
-val mod_inv_u64: n0:uint64 -> uint64
-
-val mod_inv_u64_lemma: n0:uint64 -> Lemma
-  (requires v n0 % 2 == 1)
-  (ensures (1 + v n0 * v (mod_inv_u64 n0)) % pow2 64 == 0)
 
 val precomp_r2_mod_n:
     #nLen:size_pos{128 * nLen <= max_size_t}
